\documentclass{beamer}
\usetheme{CambridgeUS}

\title{Assignment 7}
\author{Bhogalapalli Sahishnu, CS21BTECH11009}
\date{June 7, 2022}
\begin{document}

\begin{frame}
    \titlepage
\end{frame}

\section{Question}
\begin{frame}{Question}
\textbf{Papoulis-Pillai Ch 6 Ex 4-20: }\\
The random variables x and y are independent with exponential densities
\begin{align}
    f_x(x) = \alpha e^{-\alpha x} u(x) && f_y(y) = \beta e^{-\beta y} u(y)
\end{align}
Find the densities of the following random variables:
\begin{align*}
    \textbf{a)} 2x + y && \textbf{b)} x - y && \textbf{c)} \frac{x}{y} && \textbf{d)} max(x,y) && \textbf{e)} min(x,y)
\end{align*}
\end{frame}

\section{Solution}
\begin{frame}{Solution}
\textbf{a)} From the given density of x, density of 2x will be equal to $\frac{1}{2}$ $f_x(\frac{x}{2})$, Hence if $z = 2x + y$, then
\begin{align*}
    f_z(z) &= \int_{0}^{z} \frac{\alpha}{2} e^{-\alpha x/2} \beta e^{-\beta (z-x)} \,dx
\end{align*}
On integration,
\begin{align*}
    f_z(z) = \frac{\alpha \beta}{\alpha - 2\beta} (e^{\beta z} - e^{-\alpha z/2}) u(z)
\end{align*}
\end{frame}

\section{Solution}
\begin{frame}{Solution}
\textbf{b)} From the given density of y, density of -y will be equal to $f_y(-y)$. Hence if z = x - y, then 
\begin{align*}
    f_z(z) &= f_x(z)*f_y(-z)
           &= \alpha \beta    
           \begin{cases}
                \int_{z}^{\infty} e^{-\alpha x} \cdot e^{-\beta(x - z)} \, dx = \frac{\alpha \beta}{\alpha + \beta} \cdot e^{-\alpha z}, z > 0\\\\
                \int_{z}^{\infty} e^{-\alpha x} \cdot e^{-\beta(x - z)} \, dx = \frac{\alpha \beta}{\alpha + \beta} \cdot e^{\beta z}, z < 0
           \end{cases}
\end{align*}
    
\end{frame}

\section{Solution}
\begin{frame}{Solution}
\textbf{c)} z = x/y\\
Let,
\begin{align*}
    w = y && x = wz
\end{align*}
Now we can write $f_z(z)$ as 
\begin{align*}
    f_z(z) &= \alpha \beta \int_{0}^{\infty} w \cdot e^{-\alpha zw} \cdot e^{-\beta w} \, dw \\
           &= \frac{\alpha \beta}{(\alpha z + \beta)^2} u(z)
\end{align*}
\end{frame}

\section{Solution}
\begin{frame}{Solution}
\textbf{d)} z = max(x,y)\\
Here,
\begin{align}
    F_z(z) = F_{xy}(z,z) = F_x(z) \cdot F_y(z)
\end{align}
On differentiating,
\begin{align*}
    f_z(z) &= f_x(z) \cdot F_y(z) + F_x(z) \cdot f_y(z)\\\\
           &= [\alpha e^{-\alpha z}(1 - e^{-\beta z}) + \beta e^{-\beta z}(1 - e^{-\alpha z})] u(z)
\end{align*}
\end{frame}

\section{Solution}
\begin{frame}{Solution}
\textbf{e)} z = min(x,y)\\
Here,
\begin{align}
    F_z(z) = F_{x}(z) + F_{y}(z) - F_{x}(z) \cdot F_{y}(z)
\end{align}
On differentiating,
\begin{align*}
    f_z(z) &= f_x(z) \cdot [1 - F_y(z)] + f_y(z) \cdot [1 - F_x(z)]\\\\
           &= (\alpha + \beta) e^{-(\alpha + \beta)z}u(z)
\end{align*}
\end{frame}

\end{document}
